fewer word32 -> Intinf -> int conversions

Weidenbach_Book/WB_Word_Assn.thy
@@ -389,10 +389,13 @@ lemma uint32_nat_assn_less[sepref_fr_rules]:
   by sepref_to_hoare (sep_auto simp: uint32_nat_rel_def br_def max_def
       nat_of_uint32_less_iff)
 
-definition two_uint32 where \<open>two_uint32 = (2 :: nat)\<close>
+definition two_uint32_nat where [simp]: \<open>two_uint32_nat = (2 :: nat)\<close>
 
-lemma uint32_2_hnr: \<open>(uncurry0 (return 2), uncurry0 (RETURN two_uint32)) \<in> unit_assn\<^sup>k \<rightarrow>\<^sub>a uint32_nat_assn\<close>
-  by sepref_to_hoare (sep_auto simp: uint32_nat_rel_def br_def nat_of_uint32_012 two_uint32_def)
+definition two_uint32 where
+  [simp]: \<open>two_uint32 = (2 :: uint32)\<close>
+
+lemma uint32_2_hnr: \<open>(uncurry0 (return two_uint32), uncurry0 (RETURN two_uint32_nat)) \<in> unit_assn\<^sup>k \<rightarrow>\<^sub>a uint32_nat_assn\<close>
+  by sepref_to_hoare (sep_auto simp: uint32_nat_rel_def br_def nat_of_uint32_012 two_uint32_nat_def)
 
 
 text \<open>Do NOT declare this theorem as \<open>sepref_fr_rules\<close> to avoid bad unexpected conversions.\<close>
